Rename [Fail] to [Crash].
[Fail] is a Coq command. This confuses Alectryon (highlighting is wrong)
and can confuse people as well.

theories/semantics/eval.v
@@ -36,31 +36,47 @@ Implicit Type items : sitems.
    namely, pattern matching failures (caused by nonexhaustive case analyses)
    and assertion failures. *)
 
-Definition crash {A} (msg : string) : free A :=
-  fail.
-
 Definition assertion_failure {A} : free A :=
-  fail.
+  crash.
+
+Definition division_by_zero {A} : free A :=
+  crash.
+
+Definition length_mismatch {A} (msg : string) : free A :=
+  crash.
 
 Definition match_failure {A} (tt : unit) : free A :=
-  fail.
+  crash.
 
 Definition missing_field {A} (x : var) : free A :=
-  fail.
+  crash.
 
 Definition missing_variable {A} (x : var) : free A :=
-  fail.
+  crash.
 
 Definition missing_variable_or_field {A} (x : var) : free A :=
-  fail.
+  crash.
+
+Definition structural_equality_error {A} (msg : string) : free A :=
+  crash.
+
+Definition structural_ordering_error {A} (msg : string) : free A :=
+  crash.
+
+Definition type_mismatch {A} (msg : string) : free A :=
+  crash.
 
 Global Opaque
-  crash
   assertion_failure
+  division_by_zero
+  length_mismatch
   match_failure
   missing_field
   missing_variable
   missing_variable_or_field
+  structural_equality_error
+  structural_ordering_error
+  type_mismatch
 .
 
 (* ------------------------------------------------------------------------ *)
@@ -85,7 +101,7 @@ Definition val_as_bool (v : val) : free bool :=
   | VTrue =>
       ret true
   | _ =>
-      crash "type mismatch (Boolean value expected)"
+      type_mismatch "Boolean value expected"
   end.
 
 Definition as_bool (m : free val) : free bool :=
@@ -112,7 +128,7 @@ Definition val_as_loc (v: val) : free loc :=
   | VLoc l =>
       ret l
   | _ =>
-      crash "type mismatch (location value expected)"
+      type_mismatch "location value expected"
   end.
 
 Definition as_loc (m : free val) : free loc :=
@@ -128,7 +144,7 @@ Definition val_as_int (v : val) : free int :=
   | VInt i =>
       ret i
   | _ =>
-      crash "type mismatch (integer value expected)"
+      type_mismatch "integer value expected"
   end.
 
 Definition as_int (m : free val) : free int :=
@@ -138,7 +154,7 @@ Definition as_int (m : free val) : free int :=
 
 Definition check_div_by_zero i : free unit :=
   if int.eq i int.zero then
-    crash "division by zero" (* TODO raise an exception *)
+    division_by_zero (* TODO raise an exception *)
   else
     ret ().
 
@@ -153,7 +169,7 @@ Definition val_as_record (v : val) : free env :=
   | VRecord fvs =>
       ret fvs
   | _ =>
-      crash "type mismatch (record value expected)"
+      type_mismatch "record value expected"
   end.
 
 Definition as_record (m : free val) : free env :=
@@ -169,7 +185,7 @@ Definition val_as_struct (v : val) : free env :=
   | VStruct xvs =>
       ret xvs
   | _ =>
-      crash "type mismatch (structure expected)"
+      type_mismatch "structure expected"
   end.
 
 Definition as_struct (m : free val) : free env :=
@@ -395,13 +411,13 @@ Fixpoint extend δ p v : free env :=
       let i := int.repr z in
       if int.eq i i' then ret δ else next()
   | PTuple _, _ =>
-      crash "type mismatch (tuple expected)"
+      type_mismatch "tuple expected"
   | PData _ _, _ =>
-      crash "type mismatch (algebraic data expected)"
+      type_mismatch "algebraic data expected"
   | PRecord _, _ =>
-      crash "type mismatch (record expected)"
+      type_mismatch "record expected"
   | PInt _, _ =>
-      crash "type mismatch (integer expected)"
+      type_mismatch "integer expected"
   end
 
 (* [extends δ ps vs] matches the values [vs] against the patterns [ps].
@@ -423,9 +439,9 @@ with extends δ ps vs : free env :=
       δ ← extends δ ps vs ;
       ret δ
   | PCons _ _, VNil =>
-      crash "pattern matching: length mismatch (longer tuple expected)"
+      length_mismatch "longer tuple expected"
   | PNil, VCons _ _ =>
-      crash "pattern matching: length mismatch (shorter tuple expected)"
+      length_mismatch "shorter tuple expected"
   end
 
 (* [extendfs δ fps fvs] matches the field-indexed values [fvs] against the
@@ -487,7 +503,7 @@ Definition call v1 v2 : free val :=
       (* Then, proceed as in the case of a non-recursive closure. *)
       acall η a v2
    | _ =>
-      crash "type mismatch (closure expected)"
+      type_mismatch "closure expected"
    end.
 
 (* ------------------------------------------------------------------------ *)
@@ -509,7 +525,7 @@ Fixpoint eq_val v1 v2 : free bool :=
       b' ← eq_val v1 v2 ;
       ret (b && b')
   | _, _ =>
-      crash "structural equality: invalid or unsupported arguments"
+      structural_equality_error "invalid or unsupported arguments"
   end
 
 with eq_vals vs1 vs2 : free bool :=
@@ -522,7 +538,7 @@ with eq_vals vs1 vs2 : free bool :=
       ret (b && b')
   | VCons _ _, VNil
   | VNil, VCons _ _ =>
-      crash "structural equality: tuple length mismatch"
+      structural_equality_error "tuple length mismatch"
   end.
 
 Definition ne_val v1 v2 :=
@@ -550,7 +566,7 @@ Definition lt_val v1 v2 : free bool :=
       (* A signed integer comparison. *)
       ret (int.lt i1 i2)
   | _, _ =>
-      crash "structural ordering: invalid or unsupported arguments"
+      structural_ordering_error "invalid or unsupported arguments"
   end.
 
 (* The other three structural ordering operators. *)
